---
title: "Discrete Flow Matching-1"
date: 2025-07-13
categories:
  - flow-matching
permalink: /flow-matching-theorem/part-1/    
tags:
- flow matching 
- mathematics
layout: post
---



<!-- Load MathJax so LaTeX renders in GitHub Pages without touching layouts -->
<script>
  window.MathJax = {
    tex: {
      inlineMath: [['\\(','\\)'], ['\\[','\\]']]
    }
  };
</script>
<script src="https://cdn.jsdelivr.net/npm/mathjax@3/es5/tex-mml-chtml.js"></script>


## Table of Contents
- [Introduction](#introduction)
- [Training Procedure](#training-procedure)
- [Inference Procedure](#inference-procedure)
- [Factorized Source→Sink Velocities](#factorized-source-sink-velocities)




## Introduction {#introduction} 




For any smooth flow of diffeomorphisms \\(\psi_t:\mathbb{R}^d\to\mathbb{R}^d\\), define the Eulerian velocity field by

$$
u_t(x)=\dot{\psi}_t\bigl(\psi_t^{-1}(x)\bigr),
$$

where

$$
\dot{\psi}_t(y)=\frac{d}{dt}\,\psi_t(y)
=\lim_{h\to 0}\frac{\psi_{t+h}(y)-\psi_t(y)}{h}.
$$

-Autonomous Case \\(u_t \equiv u\\)}

Because the velocity is constant in time, the flow satisfies the semigroup property

$$
\psi_{t+h}=\psi_h\circ\psi_t.
$$

Hence

$$
\begin{aligned}
u(x)
&=\dot{\psi}_t\bigl(\psi_t^{-1}(x)\bigr)\\
&=\lim_{h\to0}\frac{\psi_{t+h}(\psi_t^{-1}(x))-\psi_t(\psi_t^{-1}(x))}{h}\\
&=\lim_{h\to0}\frac{(\psi_h\circ\psi_t)(\psi_t^{-1}(x))-x}{h}\\
&=\lim_{h\to0}\frac{\psi_h(x)-x}{h}.
\end{aligned}
$$

Thus in the autonomous case,

$$
u(x)
=\left.\frac{d}{dh}\right|_{h=0}\psi_h(x)
=\lim_{h\to0}\frac{\psi_h(x)-x}{h}.
$$


When \\(u_t\\) varies with time, the one‐parameter map \\(\psi_h\\) alone is not enough. Define the two‐time propagator

$$
\Phi_{t,t+h}:=\psi_{t+h}\circ\psi_t^{-1},
$$
which carries points from time \\(t\\) to \\(t+h\\). Then

$$
u_t(x)
=\lim_{h\to0}\frac{\psi_{t+h}(\psi_t^{-1}(x))-\psi_t(\psi_t^{-1}(x))}{h}
=\lim_{h\to0}\frac{\Phi_{t,t+h}(x)-x}{h}.
$$


$$
u(x) = \lim_{h \to 0} \frac{\psi_h(x) - x}{h}.
$$

$$
u_t(x) = \lim_{h \to 0} \frac{\Phi_{t,t+h}(x) - x}{h}, \quad
\Phi_{t,t+h} = \psi_{t+h}\circ\psi_t^{-1}.
$$


In both cases the compact relation

$$
u_t(x)=\dot{\psi}_t\bigl(\psi_t^{-1}(x)\bigr)
$$

holds without changing notation.